updated

Criterion/Incomplete_Criteria.thy
@@ -70,77 +70,93 @@ using decreasingPCC_imp_descentIpath scsg_limit Node_finite by blast
 
 (* 2. EXTENDED SPRENGER-DAM CRITERION  *)
 
-definition "wfLabFS Node1 lab \<equiv> \<forall>nd\<in>Node1. lab nd \<noteq> {} \<and> lab nd \<subseteq> PosOf nd"
-
-lemma wfLabFS_finite: "wfLabFS Node1 lab \<Longrightarrow> Node1 \<subseteq> Node \<Longrightarrow> nd\<in>Node1 \<Longrightarrow> finite (lab nd)" 
-unfolding wfLabFS_def using infinite_super by (metis in_mono PosOf_finite)
-
-lemma subgr_wfLabFS: 
-"subgr Node1 edge1 S2 R2 \<Longrightarrow> wfLabFS S2 lab \<Longrightarrow> wfLabFS Node1 lab"
-unfolding subgr_def subsetD wfLabFS_def by auto 
-
-definition RRSetChoice :: 
-"'node set \<Rightarrow> ('node \<Rightarrow> 'node \<Rightarrow> bool) \<Rightarrow> ('node \<Rightarrow> 'pos set) \<Rightarrow> 
-('node \<Rightarrow> 'node \<Rightarrow> 'pos \<Rightarrow> 'pos) \<Rightarrow> bool" where 
-"RRSetChoice Node1 edge1 lab f \<equiv> 
- (\<forall>nd nd'. {nd,nd'} \<subseteq> Node1 \<longrightarrow> f nd nd' ` lab nd \<subseteq> lab nd') \<and>
- (\<forall>nd nd'. {nd,nd'} \<subseteq> Node1 \<and> edge1 nd nd' \<longrightarrow> 
-   (\<forall>P \<in> lab nd. RR (nd,P) (nd',f nd nd' P) Main \<or> RR (nd,P) (nd',f nd nd' P) Decr))"
-
 (* The position-extended graph of a labeled SGSG: *)
-definition "extgrS Node1 lab \<equiv> {(nd,P). nd \<in> Node1 \<and> P \<in> lab nd}"
 
-definition "extgrR edge1 f \<equiv> 
-   \<lambda>(nd,P) (nd',P'). edge1 nd nd' \<and> f nd nd' P = P'"
+(* The global extension graph Ext(G) of the entire sloped graph: *)
+definition ExtG_Nodes :: "('node \<times> 'pos) set" where 
+"ExtG_Nodes \<equiv> {(nd, P). nd \<in> Node \<and> P \<in> PosOf nd}"
+
+definition ExtG_Edges :: "('node \<times> 'pos) \<Rightarrow> ('node \<times> 'pos) \<Rightarrow> bool" where 
+"ExtG_Edges \<equiv> \<lambda>(nd, P) (nd', P'). 
+   edge nd nd' \<and> (RR (nd,P) (nd',P') Main \<or> RR (nd,P) (nd',P') Decr)"
 
 
-lemma finite_extgrS: 
-assumes "finite Node1" "Node1 \<subseteq> Node" "wfLabFS Node1 lab"
-shows "finite (extgrS Node1 lab)"
-proof- 
-  have 0: "extgrS Node1 lab = Sigma Node1 (\<lambda>nd. lab nd)" unfolding Sigma_def extgrS_def by auto
-  show ?thesis unfolding 0 apply(rule finite_SigmaI)  
-  using assms wfLabFS_finite by blast+
-qed
-
-(* Decreasing position-change set-choice: *)
-definition decreasingPCSC :: 
+(* A Slice of a Position-change Set-choice Pi = (lab, f) w.r.t subgraph (Node1, edge1) *)
+ (* It is a subgraph of the extension graph Ext(G) *)
+(* Condition 1: Edges project to edge1 and respect the function f *)
+(* Condition 2: Every edge in the base subgraph is covered by at least one edge in the slice *)
+definition is_slice :: 
 "'node set \<Rightarrow> ('node \<Rightarrow> 'node \<Rightarrow> bool) \<Rightarrow> 
-('node \<Rightarrow> 'pos set) \<Rightarrow> ('node \<Rightarrow> 'node \<Rightarrow> 'pos \<Rightarrow> 'pos) \<Rightarrow> bool" where 
-"decreasingPCSC Node1 edge1 lab f \<equiv> 
- RRSetChoice Node1 edge1 lab f \<and> 
- (\<forall>NNode eedge. 
-     Graph.subgr NNode eedge (extgrS Node1 lab) (extgrR edge1 f) \<and> 
-     Graph.scg NNode eedge \<and>   
-     (\<forall>nd nd'. {nd,nd'} \<subseteq> Node1 \<and> edge1 nd nd' \<longrightarrow> 
-               (\<exists>P P'. {(nd,P),(nd',P')} \<subseteq> NNode \<and> eedge (nd,P) (nd',P'))) 
-     \<longrightarrow> 
-     (\<exists>nd_P nd_P'. {nd_P,nd_P'} \<subseteq> NNode \<and> eedge nd_P nd_P' \<and> 
-                   RR nd_P nd_P' Decr))"
+ ('node \<Rightarrow> 'pos set) \<Rightarrow> ('node \<Rightarrow> 'node \<Rightarrow> 'pos \<Rightarrow> 'pos) \<Rightarrow> 
+ ('node \<times> 'pos) set \<Rightarrow> (('node \<times> 'pos) \<Rightarrow> ('node \<times> 'pos) \<Rightarrow> bool) \<Rightarrow> bool" where 
+"is_slice Node1 edge1 lab f NNode eedge \<equiv> 
+  NNode \<subseteq> {(nd, P). nd \<in> Node1 \<and> P \<in> lab nd} \<and>
+  Graph.subgr NNode eedge ExtG_Nodes ExtG_Edges \<and>
+  (\<forall>nd P nd' P'. eedge (nd, P) (nd', P') \<longrightarrow> 
+     {(nd, P), (nd', P')} \<subseteq> NNode \<and> edge1 nd nd' \<and> f nd nd' P = P') \<and>
+  (\<forall>nd nd'. {nd,nd'} \<subseteq> Node1 \<and> edge1 nd nd' \<longrightarrow> 
+     (\<exists>P P'. {(nd, P), (nd', P')} \<subseteq> NNode \<and> eedge (nd, P) (nd', P')))"
 
 
-(* Extended-Sprenger-Dam (XSD) descent: *)
+(* A slice is decreasing if it contains at least one strictly decreasing edge *)
+definition decreasing_slice :: "('node \<times> 'pos) set \<Rightarrow> (('node \<times> 'pos) \<Rightarrow> ('node \<times> 'pos) \<Rightarrow> bool) \<Rightarrow> bool" where
+"decreasing_slice NNode eedge \<equiv> 
+  \<exists>nd P nd' P'. {(nd, P), (nd', P')} \<subseteq> NNode \<and> eedge (nd, P) (nd', P') \<and> RR (nd, P) (nd', P') Decr"
+
+
+(* Descending Position-Change Set-Choice using the Sliced formulation *)
+(* Every strongly connected slice of Pi is decreasing *)
+definition descending_PCSC_sliced :: 
+"'node set \<Rightarrow> ('node \<Rightarrow> 'node \<Rightarrow> bool) \<Rightarrow> 
+ ('node \<Rightarrow> 'pos set) \<Rightarrow> ('node \<Rightarrow> 'node \<Rightarrow> 'pos \<Rightarrow> 'pos) \<Rightarrow> bool" where 
+"descending_PCSC_sliced Node1 edge1 lab f \<equiv> 
+  RRSetChoice Node1 edge1 lab f \<and>
+  (\<forall>NNode eedge. 
+     is_slice Node1 edge1 lab f NNode eedge \<and> 
+     Graph.scg NNode eedge 
+     \<longrightarrow> decreasing_slice NNode eedge)"
+
+
+(* Sliced Extended-Sprenger-Dam (XSD) descent criterion: *)
 definition XSDdescending :: bool where 
-"XSDdescending \<equiv> \<forall>Node1 edge1. scsg Node1 edge1 \<longrightarrow> (\<exists>lab f. wfLabFS Node1 lab \<and> decreasingPCSC Node1 edge1 lab f)"
+"XSDdescending \<equiv> 
+  \<forall>Node1 edge1. scsg Node1 edge1 \<longrightarrow> 
+    (\<exists>lab f. wfLabFS Node1 lab \<and> descending_PCSC_sliced Node1 edge1 lab f)"
 
-lemma decreasingPCSC_imp_descentIpath: 
+
+lemma stake_sdrop_szip_nth:
+  "k < m \<Longrightarrow> stake m (sdrop j (szip A B)) ! k = (A !! (j + k), B !! (j + k))"
+  by (metis sdrop_snth snth_szip stake_nth)
+
+lemma set_stake_sdrop_szipD:
+  "(x, y) \<in> set (stake m (sdrop j (szip A B))) \<Longrightarrow> 
+   \<exists>k<m. x = A !! (j + k) \<and> y = B !! (j + k)"
+  by (metis in_set_conv_nth length_stake prod.inject
+      stake_sdrop_szip_nth)
+
+lemma eq_stake_sdrop_szip_tuple:
+  "k < m \<Longrightarrow> (x, y) = stake m (sdrop j (szip A B)) ! k \<Longrightarrow> x = A !! (j + k) \<and> y = B !! (j + k)"
+  by (metis prod.inject stake_sdrop_szip_nth)
+
+lemma descending_PCSC_sliced_imp_descentIpath: 
 assumes nds: "ipath nds" and lab: "wfLabFS (limitS nds) lab"
-and lim: "decreasingPCSC (limitS nds) (limitR nds) lab f"
+and lim: "descending_PCSC_sliced (limitS nds) (limitR nds) lab f"
 shows "\<exists>Ps. descentIpath nds Ps"
 proof-
+  (* 1. ISOLATE THE LIMIT GRAPH *)
   define Node1 edge1 where Sedge1_def: "Node1 \<equiv> limitS nds" "edge1 \<equiv> limitR nds"
   obtain n where a: "alw (holdsS Node1 aand holds2 edge1) (sdrop n nds)" 
   using ipath_ev_alw[OF Node_finite nds] unfolding ev_iff_sdrop Sedge1_def by auto
 
   define nnds where "nnds \<equiv> sdrop n nds"
-
   have lndss: "limitR nds = limitR nnds" unfolding nnds_def by auto
-
   have nnds: "ipath nnds" by (simp add: Graph.ipath_sdrop nds nnds_def)
+  
   have nnds_Sedge1: "\<forall>i. nnds!!i \<in> Node1 \<and> edge1 (nnds!!i) (nnds!!(Suc i))"
   using a unfolding nnds_def[symmetric] 
   using alw_holds2_iff_snth alw_holdsS_iff_snth alw_mono by blast
 
+  (* 2. CONSTRUCT THE POSITION STREAM Ps *)
   obtain P0 where P0: "P0 \<in> lab (shd nnds)" 
     using lab unfolding wfLabFS_def 
     by (metis Sedge1_def(1) equals0I nnds_Sedge1 snth.simps(1))
@@ -155,100 +171,195 @@ proof-
     subgoal using P0 unfolding Pi_def  
     by (metis (no_types, lifting) nnds_Sedge1 old.nat.simps(6) old.nat.simps(7) snth.simps(1))
     subgoal for i  unfolding Pi_def apply simp 
-    by (smt (verit, best) Graph.limitR_S decreasingPCSC_def 
+    by (smt (verit, best) Graph.limitR_S descending_PCSC_sliced_def 
       RRSetChoice_def Node_finite Sedge1_def(2) image_subset_iff ipath_sdrop_limit lim 
        limitR_sdrop_eq nds nnds_Sedge1) . .
 
   hence 0: "\<And>i. Ps!!i \<in> lab (nnds!!i) \<and> Ps!!(Suc i) = f (nnds !! i) (nnds !! Suc i) (Ps !! i)"  
   by (simp add: Ps_def)
-   
+    
   define \<phi> where "\<phi> \<equiv> \<lambda>i P P'. P' \<in> lab(nnds!!(Suc i)) \<and> 
             (RR (nnds!!i,P) (nnds!!(Suc i),P') Main \<or> 
              RR (nnds!!i,P) (nnds!!(Suc i),P') Decr)" 
+  
   have 2: "\<forall>i. \<phi> i (Pi i) (Pi (Suc i))" 
   using 0 unfolding \<phi>_def  
-  by (smt (verit, best) "00" decreasingPCSC_def RRSetChoice_def 
+  by (smt (verit, best) "00" descending_PCSC_sliced_def RRSetChoice_def 
          Sedge1_def(1) Sedge1_def(2) empty_subsetI insert_subset lim nnds_Sedge1) 
 
-  have nnds_Ps: "Graph.ipath (extgrS Node1 lab) (extgrR edge1 f) (szip nnds Ps)"
-  using 0 nnds_Sedge1 P0 unfolding Graph.ipath_iff_snth extgrS_def extgrR_def by auto
-
+  (* Node bounding for pigeonhole principle *)
   have Node1: "finite Node1" "Node1 \<subseteq> Node" "wfLabFS Node1 lab" 
   unfolding Sedge1_def(1) using Node_finite infinite_super limitS_S 
   apply blast by (auto simp: Sedge1_def(1) limitS_S lab)  
 
-  have eNode1: "finite (extgrS Node1 lab)" using finite_extgrS[OF Node1] .
+  (* Create a local finite state space for the pigeonhole to extract an infinite cycle *)
+  define StateSpace where "StateSpace \<equiv> {(nd, P). nd \<in> Node1 \<and> P \<in> lab nd}"
+  have eNode1: "finite StateSpace" 
+      unfolding StateSpace_def 
+    proof -
+      have "{(nd, P). nd \<in> Node1 \<and> P \<in> lab nd} = Sigma Node1 lab" by auto
+      thus "finite {(nd, P). nd \<in> Node1 \<and> P \<in> lab nd}"
+        using wfLabFS_finite[OF Node1(3) Node1(2)] Node1(1) finite_SigmaI by auto
+    qed
+    
+    
+  have ipath_states: "\<forall>i. (nnds!!i, Ps!!i) \<in> StateSpace"
+    unfolding StateSpace_def using 0 nnds_Sedge1 by auto
 
-  obtain nd P where nd_P: "(nd,P) \<in> extgrS Node1 lab" "\<forall>i. \<exists>j\<ge>i. nnds!!j = nd \<and> Ps!!j = P"
-  using Graph.ipath_infinitely_often[OF eNode1 nnds_Ps] by auto
+  obtain nd P where nd_P: "(nd,P) \<in> StateSpace" "\<forall>i. \<exists>j\<ge>i. nnds!!j = nd \<and> Ps!!j = P"
+  proof -
+    have "range (\<lambda>i. (nnds!!i, Ps!!i)) \<subseteq> StateSpace" using ipath_states by auto
+    hence fin_range: "finite (range (\<lambda>i. (nnds!!i, Ps!!i)))" 
+      using eNode1 finite_subset by auto
+      
+    obtain nd_P where "infinite {i. (nnds!!i, Ps!!i) = nd_P}"
+      using pigeonhole_infinite[OF ] fin_range by fastforce
+    moreover obtain nd P where "nd_P = (nd, P)" by fastforce
+    ultimately have inf: "infinite {i. (nnds!!i, Ps!!i) = (nd, P)}" by simp
+    
+    have "\<forall>i. \<exists>j\<ge>i. nnds!!j = nd \<and> Ps!!j = P"
+      using inf unfolding infinite_nat_iff_unbounded 
+      by (meson mem_Collect_eq order_less_imp_le prod.inject)
+    moreover have "(nd, P) \<in> StateSpace"
+      using inf ipath_states not_finite_existsD by blast
+    ultimately show ?thesis using that by blast
+  qed
 
+  (* 3. PROVE DESCENT BY EXTRACTING CYCLES *)
   have d_nnds: "descentIpath nnds Ps" 
   unfolding descentIpath_iff_snth2 apply(intro conjI)
     subgoal using 2 unfolding \<phi>_def by (simp add: Ps_def)
     subgoal proof safe
       fix i    
- 
+      (* Find next visit to (nd, P) *)
       obtain j0 where j0: "j0\<ge>i" "nnds!!j0 = nd \<and> Ps!!j0 = P" using nd_P by auto
 
+      (* Span an interval covering all edges in the limit *)
       obtain j1 j2 where j12: "j1\<ge>Suc j0" "j2\<ge>j1" 
       "\<And>nd nd'. limitR nnds nd nd' \<Longrightarrow> (\<exists>j\<ge>j1. j < j2 \<and> nnds !! j = nd \<and> nnds !! Suc j = nd')"
       using ipath_limitR_interval[OF Node_finite nnds] by blast
 
+      (* Find the subsequent visit to (nd, P) to close the cycle *)
       obtain j3 where j3: "j3\<ge>Suc j2" "nnds!!j3 = nd \<and> Ps!!j3 = P" using nd_P by auto
 
       define nd_Pl where "nd_Pl \<equiv> stake (j3-j0+1) (sdrop j0 (szip nnds Ps))"
-      have cyc: "Graph.cycleG (extgrS Node1 lab) (extgrR edge1 f) nd_Pl" 
+      
+      have cyc: "Graph.cycleG StateSpace (\<lambda>_ _. True) nd_Pl" (* Base cycle abstraction *)
       unfolding nd_Pl_def apply(rule Graph.ipath_stake_sdrop_cycle) 
-        subgoal by fact
+        subgoal by (simp add: Graph.ipath_iff_snth ipath_states)
         subgoal using j12(1) j12(2) j3(1) by linarith
         subgoal by simp (metis add_diff_cancel_left' add_leE j0(2) j12(1) j12(2) j3(1) j3(2) 
           nat_le_iff_add plus_1_eq_Suc) .
       
       define NNode where "NNode \<equiv> set (nd_Pl)"
       define eedge where "eedge \<equiv> \<lambda> nd_P nd_P'. 
-      (\<exists>i. Suc i < length nd_Pl \<and> nd_P = nd_Pl!i \<and> nd_P' = nd_Pl!(Suc i))"
+      (\<exists>k. Suc k < length nd_Pl \<and> nd_P = nd_Pl!k \<and> nd_P' = nd_Pl!(Suc k))"
 
-      have subgr: "Graph.subgr NNode eedge (extgrS Node1 lab) (extgrR edge1 f)"
-      unfolding Graph.subgr_def NNode_def eedge_def set_conv_nth  
-      using Graph.cycle_iff_nth cyc by blast
+      (* 4. VERIFY IT IS A SLICE *)
+      have subgr: "Graph.subgr NNode eedge ExtG_Nodes ExtG_Edges"
+        unfolding Graph.subgr_def NNode_def eedge_def ExtG_Nodes_def ExtG_Edges_def
+        apply safe
+        subgoal for nd P 
+          unfolding nd_Pl_def
+          apply (drule set_stake_sdrop_szipD)
+          using ipath_iff_snth nnds StateSpace_def by fastforce
+        subgoal for nd P 
+          unfolding nd_Pl_def
+          apply (drule set_stake_sdrop_szipD)
+          using ipath_states Node1(3) unfolding StateSpace_def wfLabFS_def 
+          by auto
+        subgoal for nd P nd' P' k
+          apply(rule ssubst[of "nd" "nnds !! (j0 + k)"])
+          apply (metis Suc_lessD length_stake nd_Pl_def prod.inject stake_sdrop_szip_nth)
+          apply(rule ssubst[of "nd'" "nnds !! Suc (j0 + k)"])
+          apply (unfold nd_Pl_def, metis prod.inject stake_sdrop_szip_nth nd_Pl_def length_stake add_Suc_right)
+          using ipath_iff_snth nnds by blast
+        subgoal for nd P nd' P' k
+          apply(rule ssubst[of "(nd,P)" "(nnds !! (j0 + k), Ps !! (j0 + k))"])
+           apply(unfold nd_Pl_def, metis Suc_lessD length_stake sdrop_snth snth_szip stake_nth)
+          apply(rule ssubst[of "(nd', P')" "(nnds !! Suc (j0 + k), Ps !! Suc (j0 + k))"])
+          apply( metis add_Suc_right length_stake sdrop_snth snth_szip stake_nth)
+          using 2[THEN spec, of "j0 + k"] 
+          unfolding nd_Pl_def \<phi>_def Ps_def 
+          by (metis Suc_lessD add_Suc_right length_stake snth_fToStream
+              stake_sdrop_szip_nth) .
 
+      have proj: "\<forall>x P y P'. eedge (x, P) (y, P') \<longrightarrow> {(x, P), (y, P')} \<subseteq> NNode \<and> edge1 x y \<and> f x y P = P'"
+        unfolding eedge_def apply clarify
+        subgoal for x P y P' k
+          using nnds_Sedge1[THEN spec, of "j0 + k"] 0[of "j0 + k"]
+          unfolding nd_Pl_def 
+          by (metis Suc_lessD add_Suc_right eq_stake_sdrop_szip_tuple
+              length_stake NNode_def Suc_lessD empty_subsetI in_set_conv_nth insert_subset nd_Pl_def) .
+
+      have cover: "\<forall>x y. {x, y} \<subseteq> Node1 \<and> edge1 x y \<longrightarrow> 
+                   (\<exists>P P'. {(x,P),(y,P')} \<subseteq> NNode \<and> eedge (x,P) (y,P'))"
+      unfolding NNode_def eedge_def Sedge1_def lndss
+      proof clarify
+        fix x y
+        assume nodes: "{x, y} \<subseteq> limitS nds"
+        assume edge: "limitR nnds x y"
+
+        (* Extract the interval index j where the edge is traversed *)
+        from j12(3)[OF edge] obtain j where j_bound: "j1 \<le> j" "j < j2"
+          and x_eq: "x = nnds !! j" and y_eq: "y = nnds !! Suc j" by blast
+
+        define k where "k \<equiv> j - j0"
+
+        (* Prove arithmetic bounds *)
+        have j0_j: "j0 \<le> j" using j12(1) j_bound(1) by linarith
+        have k_len1: "k < j3 - j0 + 1" and k_len2: "Suc k < j3 - j0 + 1"
+          unfolding k_def using j12(1) j_bound(2) j3(1) j0_j by linarith+
+        have len_Pl: "length nd_Pl = j3 - j0 + 1" unfolding nd_Pl_def by simp
+
+        (* Extract the k and (Suc k) elements instantly using the helper lemma *)
+        have nth_k: "nd_Pl ! k = (x, Ps !! j)"
+          unfolding nd_Pl_def k_def using j0_j k_len1 
+          by (metis Nat.add_diff_assoc add_diff_cancel_left' k_def
+              stake_sdrop_szip_nth x_eq)
+        have nth_Suc_k: "nd_Pl ! Suc k = (y, Ps !! Suc j)"
+          unfolding nd_Pl_def k_def using j0_j k_len2 
+          by (metis Nat.add_diff_assoc add_Suc_right add_diff_cancel_left'
+              k_def stake_sdrop_szip_nth y_eq)
+
+        show "\<exists>P P'. {(x, P), (y, P')} \<subseteq> set nd_Pl \<and>
+                     (\<exists>i. Suc i < length nd_Pl \<and> (x, P) = nd_Pl ! i \<and> (y, P') = nd_Pl ! Suc i)"
+        proof (intro exI2[of _ "Ps !! j" "Ps !! Suc j"] conjI)
+          show "{(x, Ps !! j), (y, Ps !! Suc j)} \<subseteq> set nd_Pl"
+            using nth_k nth_Suc_k k_len1 k_len2 len_Pl nth_mem by (metis empty_subsetI insert_subset)
+          show "\<exists>i. Suc i < length nd_Pl \<and> (x, Ps !! j) = nd_Pl ! i \<and> (y, Ps !! Suc j) = nd_Pl ! Suc i"
+            using k_len2 nth_k nth_Suc_k len_Pl by (metis exI[of _ k])
+        qed
+      qed
+
+      have nnode_bound: "NNode \<subseteq> {(nd, P). nd \<in> Node1 \<and> P \<in> lab nd}"
+        unfolding NNode_def StateSpace_def[symmetric]
+      proof
+        fix x assume "x \<in> set nd_Pl"
+        then obtain k where "x = nd_Pl ! k" "k < length nd_Pl" 
+          by (metis \<open>x \<in> set nd_Pl\<close> in_set_conv_nth)
+        thus "x \<in> StateSpace"
+          unfolding nd_Pl_def using ipath_states
+          by (metis length_stake sdrop_snth snth_szip stake_nth)
+      qed
+
+      have is_slice: "is_slice Node1 edge1 lab f NNode eedge"
+      unfolding is_slice_def using subgr proj cover nnode_bound by blast
+
+      (* 5. APPLY THE CRITERION *)
       have scg: "Graph.scg NNode eedge" apply(subst Graph.scg_iff_cycle)
         subgoal unfolding NNode_def by auto
         subgoal unfolding NNode_def 
-        by simp (metis Graph.cycle_iff_nth cyc less_nat_zero_code list.size(3) 
-         not_path_Nil path_iff_nth)
+        by simp (metis Graph.cycle_iff_nth cyc less_nat_zero_code list.size(3) not_path_Nil path_iff_nth)
         subgoal apply(rule exI[of _ nd_Pl], standard)
           subgoal using cyc unfolding Graph.cycleG_def NNode_def eedge_def 
              unfolding Graph.path_iff_set_nth by auto
           subgoal unfolding NNode_def .. . .
 
-      have "\<forall>nd nd'. edge1 nd nd' \<longrightarrow> 
-        (\<exists>i<length nd_Pl - 1. \<exists>P P'. nd_Pl ! i = (nd, P) \<and> nd_Pl ! Suc i = (nd', P'))" 
-      apply safe unfolding Sedge1_def lndss apply(drule j12(3)) apply safe
-         subgoal for nd nd' j 
-         apply(rule exI[of _ "j-j0"]) apply safe
-           subgoal unfolding nd_Pl_def using j12(1) j3(1) by auto
-           subgoal apply(rule exI[of _ "Ps!!j"]) apply(rule exI[of _ "Ps!!(Suc j)"])
-           unfolding nd_Pl_def apply safe
-             subgoal apply(subst stake_nth)
-               subgoal using j3(1) by linarith
-               subgoal unfolding sdrop_snth 
-                 by (metis Suc_leD j12(1) le_add_diff_inverse le_trans snth_szip) .
-             subgoal apply(subst stake_nth)
-               subgoal using j3(1)j12(1) by linarith
-               subgoal unfolding sdrop_snth 
-                 by (metis Suc_leD add_Suc_right j12(1) le_add_diff_inverse le_trans snth_szip) . . . .  
-
-      hence "(\<forall>nd nd'. edge1 nd nd' \<longrightarrow> 
-               (\<exists>P P'. {(nd,P),(nd',P')} \<subseteq> NNode \<and> eedge (nd,P) (nd',P')))"
-      unfolding NNode_def eedge_def  
-      by simp (smt (verit, best) Suc_less_eq Suc_pred diff_is_0_eq' 
-         gr_zeroI less_Suc_eq less_imp_le_nat nth_mem)
-
-      with subgr scg obtain nd_P nd_P' where 
-      "{nd_P,nd_P'} \<subseteq> NNode \<and> eedge nd_P nd_P'"
-      "RR nd_P nd_P' Decr"
-      using lim unfolding decreasingPCSC_def Sedge1_def[symmetric] by metis
+      with is_slice lim obtain nd_d P_d nd_d' P_d' where 
+      decr_edge: "eedge (nd_d, P_d) (nd_d', P_d')" "RR (nd_d, P_d) (nd_d', P_d') Decr"
+      unfolding descending_PCSC_sliced_def decreasing_slice_def 
+      by (metis scg Sedge1_def(2) Sedge1_def(1))
 
       then obtain k where k: "k<length nd_Pl - 1" "RR (nd_Pl ! k) (nd_Pl ! Suc k) Decr"
       by (metis Suc_lessE diff_Suc_1 eedge_def) 
@@ -264,14 +375,86 @@ proof-
   show ?thesis using d_nnds by (simp add: descentIpath_sdrop_any nnds_def)
 qed
 
-
 proposition XSDdescending_implies_InfiniteDescent: 
-"XSDdescending \<Longrightarrow> InfiniteDescent"
-unfolding XSDdescending_def InfiniteDescent_def 
-using decreasingPCSC_imp_descentIpath scsg_limit Node_finite by blast
+  "XSDdescending \<Longrightarrow> InfiniteDescent"
+  unfolding XSDdescending_def InfiniteDescent_def 
+  using descending_PCSC_sliced_imp_descentIpath scsg_limit Node_finite by blast
 
 lemmas Incomplete_Criterion = SDdescending_imp_InfiniteDescent 
                               XSDdescending_implies_InfiniteDescent
+
+(**SD implies XSD**)
+theorem SDdescending_implies_XSDdescending:
+  "SDdescending \<Longrightarrow> XSDdescending"
+  unfolding SDdescending_def XSDdescending_def
+proof clarify
+  fix Node1 edge1
+  assume SD: "\<forall>Node1 edge1. scsg Node1 edge1 \<longrightarrow> (\<exists>lab. wfLabF Node1 lab \<and> decreasingPCC edge1 lab)"
+  assume scsg: "scsg Node1 edge1"
+  
+  (* 1. Sanitize the edge relation to guarantee strict node inclusion *)
+  define edge1' where "edge1' \<equiv> \<lambda>x y. edge1 x y \<and> x \<in> Node1 \<and> y \<in> Node1"
+  
+  have scsg': "scsg Node1 edge1'"
+    using scsg Graph_scg_restrict unfolding scsg_def edge1'_def Graph.subgr_def
+    by auto
+    
+  (* 2. Apply SDdescending to the sanitized subgraph *)
+  from SD scsg' obtain lab where wf: "wfLabF Node1 lab" and pcc: "decreasingPCC edge1' lab"
+    by blast
+    
+  (* 3. Construct XSD witnesses (Singletons) *)
+  define lab' where "lab' \<equiv> \<lambda>nd. {lab nd}"
+  define f where "f \<equiv> \<lambda>(nd::'node) nd' (P::'pos). lab nd'"
+  
+  show "\<exists>lab' f. wfLabFS Node1 lab' \<and> descending_PCSC_sliced Node1 edge1 lab' f"
+  proof (intro exI conjI)
+    show "wfLabFS Node1 lab'"
+      using wf unfolding wfLabF_def wfLabFS_def lab'_def by blast
+      
+    show "descending_PCSC_sliced Node1 edge1 lab' f"
+      unfolding descending_PCSC_sliced_def 
+    proof (intro conjI allI impI)
+      (* A: RRSetChoice *)
+      show "RRSetChoice Node1 edge1 lab' f"
+        using pcc unfolding decreasingPCC_def RRSetChoice_def lab'_def f_def edge1'_def by auto
+        
+      (* B: The Slice Condition *)
+      fix NNode eedge
+      assume "is_slice Node1 edge1 lab' f NNode eedge \<and> Graph.scg NNode eedge" 
+      hence  is_slice: "is_slice Node1 edge1 lab' f NNode eedge"
+         and scg: "Graph.scg NNode eedge" by auto
+                     
+      (* 1. Obtain the decreasing edge, GUARANTEED to be in Node1 thanks to edge1' *)
+      from pcc obtain nd_d nd_d' where decr: "edge1' nd_d nd_d'" "RR (nd_d, lab nd_d) (nd_d', lab nd_d') Decr"
+        unfolding decreasingPCC_def by blast
+        
+      have nodes_in: "{nd_d, nd_d'} \<subseteq> Node1" and orig_edge: "edge1 nd_d nd_d'"
+        using decr(1) unfolding edge1'_def by auto
+        
+      (* 2. Force the slice to cover this specific decreasing edge *)
+      have cover: "\<forall>x y. {x, y} \<subseteq> Node1 \<and> edge1 x y \<longrightarrow> 
+                   (\<exists>P P'. {(x, P), (y, P')} \<subseteq> NNode \<and> eedge (x, P) (y, P'))"
+        using is_slice unfolding is_slice_def by blast
+        
+      obtain P P' where in_slice: "{(nd_d, P), (nd_d', P')} \<subseteq> NNode" "eedge (nd_d, P) (nd_d', P')"
+        using cover nodes_in orig_edge by blast
+        
+      (* 3. Extract the exact positions from the singleton sets *)
+      have nnode_bound: "NNode \<subseteq> {(nd, P). nd \<in> Node1 \<and> P \<in> lab' nd}"
+        using is_slice unfolding is_slice_def by auto
+
+      have "P = lab nd_d" and "P' = lab nd_d'"
+        using in_slice(1) nnode_bound unfolding lab'_def by auto
+        
+      (* 4. Output the final existential witnesses for decreasing_slice *)
+      show "decreasing_slice NNode eedge"
+        unfolding decreasing_slice_def
+        using in_slice decr(2) \<open>P = lab nd_d\<close> \<open>P' = lab nd_d'\<close> by blast
+    qed
+  qed
+qed
+
 end (* context Sloped_Graph *) 
 
 
