README.md
@@ -27,47 +27,58 @@ Sloped_Graphs.thy:
 
 Subfolders and their contents:
 
-docs: 
+HTML: 
     A folder containing the browsable HTML version of each Isabelle file contained in this folder
 
 Criterion:
     The development of each criterion outlined in the paper
 
     -- VLA_Criterion.thy:
-        Imports the Buchi_Preliminaries file to mechanize the VLA Criterion, as seen in Section 3.1 (Definition 4 & 5 and Theorem 6).
+        Imports the Buchi_Preliminaries file to mechanize the VLA Criterion, as seen in Section 3.1.1 (Definition 4 & 5, Theorem 6).
 
     -- SLA_Criterion.thy:
-        Imports the Buchi_Preliminaries file to mechanize the SLA Criterion, as seen in Section 3.1 (Definition 7 & 8 and Theorem 9). 
-        
-    -- Relation_Based_Criterion.thy:
-        Definitions related to, and completeness proof of the relation based criterion as seen in Section 3.2 (Definition 10 and Theorem 11).
+        Imports the Buchi_Preliminaries file to mechanize the SLA Criterion, as seen in Section 3.1.2 (Definition 7 & 8, Theorem 9). 
 
     -- Incomplete_Criteria.thy:
-        Definitions and soundness proofs of the (Extended) Sprenger-Dam Criteria as seen in Section 4.1 (Definition 12, 14, 15 & 16 and Prop. 13 & 17).
-        
-    -- SD_Incomplete.thy:
-        A demonstration of incompleteness for the Sprenger-Dam Criterion, as described in Section 4.1.2.
+        Definitions and soundness proofs of the (Extended) Sprenger-Dam Criteria as seen in Section 4.1 (Definition 10, 13 & 14 and Prop. 11 & 15).
+	We also include a proof that SD implies XSD by showing how the former is a specific case of the later
 
-    -- XSD_Incomplete.thy:
-        A demonstration of incompleteness for the Extended Sprenger-Dam Criterion, as described in  Section 4.1.1 (Example 18).
+    -- Relation_Based_Criterion.thy:
+        Definitions related to, and completeness proof of the relation based criterion as seen in Section 4.2 (Definition 17, 19 & 21, Proposition 18 & 20, and Theorem 22).
 
     -- Flat_Cycles_Criterion.thy:
-        A proof of soundness for the Flat Cycles criterion as seen in Section 4.2 (Theorem 19)
+        A proof of soundness for the Flat Cycles criterion as seen in Section 5.1 (Theorem 23)
 
     -- Descending_Unicycles_Criterion.thy:
-        A proof of (relative) completeness for the Descending Unicycles criterion as seen in Section 5.1 (Definition 20 & 21 and Theorem 22)
+        A proof of (relative) completeness for the Descending Unicycles criterion as seen in Section 5.1 (Definition 25 & 26 and Theorem 27)
 
     -- All.thy:
         Imports all of the above criterion to make each available for a given instantiation, this is the main theory to import.
 
+    -- Incompleteness
+	-- SD_Incomplete.thy:
+       	   A demonstration of incompleteness for the Sprenger-Dam Criterion, as described in Section 4.1 (Example 12).
 
+    	-- XSD_Incomplete.thy:
+           A demonstration of incompleteness for the Extended Sprenger-Dam Criterion, as described in  Section 4.1 (Example 16).
 
+    -- OXSD
+	-- OXSD_Criterion.thy:
+	   An alternative legacy definition of the Extended Sprenger-Dam Criterion (OXSD -- Old Extended Sprenger Dam) 
+	   this definiton was presented in the first iteration of this work, and later refactored into the "sliced" version presented in the paper
+	   To give confidence in our refactorisation we include this definition to show equivalence between the two.
+
+	-- OXSD_Incomplete.thy:
+	   A demonstration (identical to the one shown in the paper & XSD_incomplete) that this definition is also incomplete
+
+	-- XSD_Equivalence.thy
+	   Equivalence proofs between OXSD and XSD, as well as a result that SD implies OXSD.
 
 Examples:
     A collection of concrete instantiations of the Sloped Graph locale, and (dis)proofs of Infinite Descent.
 
     -- Flat_Aux.thy:
-        The instantiation of the Flat_Aux call graph as detailed in Section 2.3. (Figure 1)
+        The instantiation of the Flat_Aux call graph as detailed in Section 2.3. (Figure 2)
 
     -- Flat_Aux_SLA.thy:
         A demonstration of Infinite Descent proved for Flat_Aux sloped graph using the SLA criterion.
@@ -79,28 +90,23 @@ Examples:
         A disproof of Infinite Descent using the Flat Cycles Criterion seen in Section 5.1 (Example 24). This example is Fig. 4b from "Cyclone: A Heterogeneous Tool for Verifying Infinite Descent" - Cohen et al.
 
     -- Descending_Unicycles_Example.thy:
-        A proof of Infinite Descent using the Descending Unicycles Criterion described in Section 5.1. Namely Fig. 6a from "Cyclone: A Heterogeneous Tool for Verifying Infinite Descent" - Cohen et al. This theory also verifies that this graph does not satisfy the Flat Cycles criterion.
+        A proof of Infinite Descent using the Descending Unicycles Criterionseen in Section 5.2 (Example 28). Namely Fig. 6a from "Cyclone: A Heterogeneous Tool for Verifying Infinite Descent" - Cohen et al. This theory also verifies that this graph does not satisfy the Flat Cycles criterion.
 
     -- Descending_Unicycles_CounterExample.thy:
-        A disproof of Infinite Descent using the Descending Unicycles Criterion described in Section 5.1. Namely Fig. 6b from "Cyclone: A Heterogeneous Tool for Verifying Infinite Descent" - Cohen et al.
+        A disproof of Infinite Descent using the Descending Unicycles Criterion seen in Section 5.2 (Example 29). Namely Fig. 6b from "Cyclone: A Heterogeneous Tool for Verifying Infinite Descent" - Cohen et al.
         
 ### How to run, and browsable version ###
 
-The folder includes the source (theory) files, which can be run with the latest version of Isabelle, namely Isabelle2025-2, available for download from 
+The folder includes the source (theory) files, which can be run with the latest version of Isabelle, namely Isabelle2025, available for download from 
 [https://isabelle.in.tum.de/](https://isabelle.in.tum.de/)
 
-The formalization depends on the Buchi_Complementation AFP entry, as such the AFP must also be installed and correctly configured. To do so download the latest AFP from:
-https://www.isa-afp.org/download/
-and refer to it as a component as described here:
-https://www.isa-afp.org/help/
-
-The theory scripts can then be inspected by opening Isabelle in interactive mode. They can also be processed in batch mode using the command
+The theory scripts can be inspected by opening Isabelle in interactive mode. They can also be processed in batch mode using the command
 
 `isabelle build -D . -v`
 
 where "isabelle" is an alias for 
 the full path to the Isabelle2025 executable. (Details on how to download/install Isabelle and locale the Isabelle executable are operating-system specific and can be found on the [installation instructions from the Isabelle website](https://isabelle.in.tum.de/installation.html)).
 
-The archive also contains a browsable (html) version of the theories, located in the subfolder `docs`. The entry point for navigation is, as usual, the file index.html. The command we used to produce these is
+The archive also contains a browsable (html) version of the theories, located in the subfolder `Browsable`. The entry point for navigation is, as usual, the file index.html. The command we used to produce these is
 
 `isabelle build -D . -o browser_info -v`
